src/arch/x64/printGcc.s.dfy
@@ -215,7 +215,6 @@ method printIns(ins:ins)
         case Sub32(dst, src)    => printName2("  sub", dst, src); printOprnd(src); print(", "); printOprnd(dst); print("\n");
         case Mul32(src)         => printName1("  mul", src);      printOprnd(src); print("\n");
         case AddCarry(dst, src) => printName2("  add", dst, src); printOprnd(src); print(", "); printOprnd(dst); print("\n");
-        case BSwap32(dst)       => printName1("  bswap", dst);    printOprnd(dst); print("\n");
         case Xor32(dst, src)    => printName2("  xor", dst, src); printOprnd(src); print(", "); printOprnd(dst); print("\n");
         case Xor64(dst, src)    => printName2("  xor", dst, src); printOprnd(src); print(", "); printOprnd(dst); print("\n");
         case And32(dst, src)    => printName2("  and", dst, src); printOprnd(src); print(", "); printOprnd(dst); print("\n");
